
%>=====<  Question 10 >=====<%

\question
State and prove the theorem regarding properties of measures. Why the two continuity properties
are called in this way? For what concerns continuity w.r.t. a descending sequence ${E_k}$, show that
the hypothesis $\mu(E_1) < +\infty$ is essential.

\subsection*{Solution}
\subsection{Properties of measures}
Let us state and prove the properties of a measure $\mu$ on a set $X$ and $\salg$ $\A$:
\begin{enumerate}[i)]
    \item \label{meas:add} \textbf{Additivity:} \\
    $\forall \{ E_1, \dots, E_n \} \subseteq \A$ disjoint we have:
    \[
        \mu\left( \bigcup_{k=1}^{n} E_k \right) = \sum_{k=1}^{n} \mu(E_k)
    \]
    \begin{proof}
    indeed if we define a sequence such that:
    \[
        \seq{E} = \left\{ \begin{array}{l}
            B_k = E_k \quad \forall k \leq n\\
            B_k = \emptyset \quad \forall k > n
        \end{array} \right.
    \]
    this sequence is also disjoint ($E\cap\emptyset = \emptyset$ $\forall E\in X$), thus we may write:
    \[
        \mu \underbrace{ \left( \bigcup_{k=1}^{\infty} E_k \right) }_{=\bigcup_{k=1}^{n} E_k \cup \emptyset}
         = \sum_{k=1}^{\infty} \mu(E_k) = \sum_{k=1}^{n} \mu(E_k) + \sum_{k=n+1}^{\infty} \underbrace{\cancelnum{}{\mu(E_k)}}_{=0}
    \]
    \end{proof}

    \item \label{meas:mono} \textbf{Monotonicity:} \\
    $\forall E,F \in \A$ we have:
    \[
        E\subseteq F \implies \mu(E) \leq \mu(F)    
    \]
    \begin{proof}
    We may write $F$ in the following way:
    \[
        F=E\cup (F \setminus E) 
    \]
    and since these two sets are obviously disjoint we may use (\ref{meas:add}) to write:
    \[
        \mu(F) = \mu(E)+\underbrace{\mu(E \setminus F)}_{\geq 0} > \mu(E)
    \]
    \end{proof}
    
    \item \label{meas:sub} \textbf{$\s{subadditivity}$:} \\
    $\forall \seq{E}\subseteq\A$ (\textbf{not} disjoint) we have:
    \[
        \mu\left( \bigcup_{k=1}^{\infty} E_k \right) \leq \sum_{k=1}^{\infty} \mu(E_k)
    \]
    \begin{proof}
    \provdef{}
    \[
        \left\{ \begin{array}{l}
            F_1 \coloneqq E_1 \\
            F_n \coloneqq E_n \setminus \bigcup_{k=1}^{n-1} E_k \quad \forall n > 1
        \end{array} \right.  
    \]
    Clearly $\seq{F} \subseteq \A$ and $\seq{F}$ is a disjoint sequence and:
    \[
        \begin{array}{l}
            F_k \subseteq E_k \quad \forall k\in\N \implies \mu(F_k) \leq \mu(E_k) \text{ by (\ref{meas:mono})} \\
            \bigcup_{k=1}^{\infty} F_k = \bigcup_{k=1}^{\infty} E_k    
        \end{array}
    \]
    thus we may write:
    \[
        \mu\left( \bigcup_{k=1}^{\infty} E_k \right) = \mu\left( \bigcup_{k=1}^{\infty} F_k \right) = \sum_{k=1}^{\infty} \mu(F_k) \leq \sum_{k=1}^{\infty} \mu(E_k)   
    \]
    \end{proof}

    \item \label{meas:contbel} \textbf{Continuity from below:} \\
    $\forall \seq{E}\subseteq\A, \; E_k \nearrow$ we have:
    \[
        \mu \left( \lim_{k\to\infty}E_k \right)  = \lim_{k\to\infty} \mu(E_k)    
    \]
    \begin{proof}
    \provdef[a new sequence $\seq{F}$]
    \[
        \left\{ \begin{array}{l}
            F_k \coloneqq E_k \setminus E_{k-1} \quad \forall k \in\N \text{ and } E_0 \coloneqq \emptyset \\
            \implies \bigcup_{k=1}^n F_k = E_n ,\; \bigcup_{k=1}^{\infty} F_k = \bigcup_{k=1}^{\infty} E_k
        \end{array} \right.
    \]
    and since $\seq{F}$ is a disjoint sequence (we may visually think of it as a set of ever increasing rings) we may use (\ref{meas:add}) to write:
    \begin{align*}
        \mu\left( \lim_{n\to\infty} E_n \right) &\tikzmarknode{eq1}{=} \mu\left( \bigcup_{k=1}^{\infty} E_k \right) = \mu\left( \bigcup_{k=1}^{\infty} F_k \right) \\
        & \tikzmarknode{eq2}{=} \lim_{n\to\infty}\sum_{k=1}^{n} \mu(F_k) = \lim_{n\to\infty} \mu \left( \bigcup_{k=1}^{n} F_k \right) \\
        & \tikzmarknode{eq3}{=} \lim_{n\to\infty} \mu(E_n)
    \end{align*} \tikz[overlay,remember picture]{\draw[shorten >=1pt,shorten <=1pt] (eq1) -- (eq2) -- (eq3);}
    \end{proof}

    \item \label{meas:contab} \textbf{Continuity from above:} \\
    $\forall \seq{E} \subseteq \A$, $E_k\searrow$, $\mu(E_1) < +\infty$ we have:
    \[
        \mu\left( \lim_{n\to\infty} E_n \right) = \lim_{n\to\infty} \mu(E_n)
    \]
    \begin{proof}
    Like we did above \provdef{a new sequence $\seq{F}$}
    \[
            F_k \coloneqq E_1 \setminus E_k \quad \forall k \in\N
    \]
    let us note that $\seq{F}$ is an increasing sequence thus by (\ref{meas:contbel}) we can write:
    \[
        \mu\left( \bigcup_{k=1}^{\infty} F_k \right) = \lim_{k\to\infty} \mu(F_k) = \mu(E_1) - \lim_{k\to\infty}  (E_k)   
    \]
    because by (\ref*{meas:mono}) $\mu(F \setminus E) = \mu(F)-\mu(E)$, moreover:
    \begin{align*}
        \bigcup_{k=1}^{\infty} F_k & = \bigcup_{k=1}^{\infty} (E_1\cap E_k^\complement) = E_1\cap \left( \bigcup_{k=1}^{\infty} E_k^\complement \right) = E_1 \setminus \left( \bigcap_{k=1}^{\infty} E_k \right) \\
        &\implies \mu\left( \bigcup_{k=1}^{\infty} F_k \right) = \mu(E_1) - \mu \left( \bigcap_{k=1}^{\infty} E_k \right)
    \end{align*}
    thus combining these two and canceling the $\mu(E_1)$ on both sides we obtain:
    \[
        \lim_{k\to\infty} \mu(E_k) = \mu \left( \bigcap_{k=1}^{\infty} E_k \right)
    \]
    \end{proof}
    let us note that for this last, crucial, step $\mu(E_1)$ must be finite, otherwise we would not be able to cancel it out from both sides.
\end{enumerate}